swap example: cleanup

bedrock2/src/Examples/Swap.v
@@ -22,116 +22,58 @@ Example swap_c_string := Eval compute in
   BasicC64Syntax.c_func "swap" swap.
 (* Print swap_c_string. *)
 
-Require Import bedrock2.BasicC64Semantics bedrock2.Map.
+Import List.ListNotations.
+Require Import bbv.Word.
+Require Import bedrock2.Semantics bedrock2.BasicC64Semantics bedrock2.Map.
 Require Import bedrock2.WeakestPrecondition.
 Require Import bedrock2.Map.Separation bedrock2.Map.SeparationLogic.
-Import List.ListNotations Word.
 
 Lemma get_sep {key value} {map : map key value} (a:key) (v:value) R m (H : sep (ptsto a v) R m) : map.get m a = Some v.
 Admitted.
 Lemma put_sep {key value} {map : map key value} (k:key) (v1:value) (v2:value) R m :
   sep (ptsto k v1) R m -> sep (ptsto k v2) R (map.put m k v2).
 Admitted.
-Lemma split_combine n a b : Semantics.split n (Semantics.combine n a b) = (a, b).
+Lemma split_combine n a b : split n (Semantics.combine n a b) = (a, b).
 Admitted.
+
+Definition ptsto sz a v m := m = unchecked_store sz map.empty a v.
+Lemma load_sep sz a v R m (H : sep (ptsto sz a v) R m) : load sz m a = Some v.
+Admitted.
+Lemma store_sep sz a v1 v2 R m (H : sep (ptsto sz a v1) R m)
+      (Q : _ -> Prop) (HQ : forall m', sep (ptsto sz a v2) R m' -> Q m') :
+  exists m', store sz m a v2 = Some m' /\ Q m'.
+Admitted.
+
+Ltac sep m Hm :=
+  revert Hm; revert m;
+  lazymatch goal with |- forall (x:?T), ?A x -> ?B x => change (@Lift1Prop.impl1 T A B) end;
+  cancel; reflexivity.
+Ltac intros_mem m Hm :=
+  let m' := fresh in let Hm' := fresh in
+  intros m' Hm'; clear m Hm; rename m' into m; rename Hm' into Hm.
+Ltac t :=
+  let m := lazymatch goal with m : @map.rep word byte mem |- _ => m end in
+  let Hm := lazymatch goal with Hm : _ m |- _ => Hm end in
+  lazymatch goal with |- load ?sz ?m ?a = Some _
+    => lazymatch type of Hm with context [ptsto sz a ?v]
+                             (* FIXME this VV Hm is dynamically scoped, not the Hm above *)
+    => refine (load_sep sz a v ltac:(clear Hm m) m ltac:(sep m Hm)) end
+  | |- exists _, store ?sz ?m ?a ?v2 = Some _ /\ _
+    => lazymatch type of Hm with context [ptsto sz a ?v1]
+    => refine (store_sep sz a v1 v2 ltac:(clear m Hm) m ltac:(sep m Hm) _ ?[cont]); intros_mem m Hm end
+  | _ => first [ eassumption | eexists | subst; eexists ]
+end.
 
 Goal
   map.ok Semantics.mem ->
   forall a_addr a b_addr b (m:map.rep (value:=@Semantics.byte _)) R t,
-    (sep (ptsto a_addr a) (sep (ptsto b_addr b) R)) m ->
+    (sep (ptsto 1 a_addr a) (sep (ptsto 1 b_addr b) R)) m ->
   WeakestPrecondition.func
     (fun _ => True) (fun _ => False) (fun _ _ => True) (fun _ _ _ _ _ => False)
     (@swap BasicC64Syntax.parameters) t m (a_addr::b_addr::nil)
-    (fun t' m' rets => t=t' /\ (sep (ptsto a_addr b) (sep (ptsto b_addr a) R)) m' /\ rets = nil).
+    (fun t' m' rets => t=t' /\ (sep (ptsto 1 a_addr b) (sep (ptsto 1 b_addr a) R)) m' /\ rets = nil).
 Proof.
-  intros.
-  eexists.
-  eexists.
-  eexists.
-  eexists.
-  eexists.
-  eexists.
-  eexists.
-  eexists.
-
-  change (BinIntDef.Z.to_nat 1) with 1%nat.
-  unfold Semantics.load.
-  unshelve erewrite (get_sep b_addr b); shelve_unifiable. reflexivity.
-  revert H0. generalize m.
-  instantiate (1 := ltac:(clear H0 m)).
-  lazymatch goal with |- forall (x:?T) (H:?A x), ?B x => change (@Lift1Prop.impl1 T A B) end.
-  cancel. reflexivity.
-
-  eexists.
-  eexists.
-  subst; eexists.
-  eexists.
-  eexists.
-  eexists.
-  eexists.
-  subst; eexists.
-
-  change (BinIntDef.Z.to_nat 1) with 1%nat.
-  unfold Semantics.load.
-  unshelve erewrite (get_sep a_addr a); shelve_unifiable. reflexivity.
-  revert H0. generalize m.
-  instantiate (1 := ltac:(clear H0 m)).
-  lazymatch goal with |- forall (x:?T) (H:?A x), ?B x => change (@Lift1Prop.impl1 T A B) end.
-  cancel. reflexivity.
-  
-  eexists.
-  eexists.
-
-  change (BinIntDef.Z.to_nat 1) with 1%nat.
-  unfold Semantics.store.
-  rewrite split_combine.
-  unshelve erewrite (get_sep b_addr b); shelve_unifiable. reflexivity.
-  revert H0. generalize m.
-  instantiate (1 := ltac:(clear H0 m)).
-  lazymatch goal with |- forall (x:?T) (H:?A x), ?B x => change (@Lift1Prop.impl1 T A B) end.
-  cancel. reflexivity.
-  intros.
-  unshelve (let pf := open_constr:(put_sep b_addr b a _ m _) in pose proof pf); shelve_unifiable.
-  revert H0.
-  generalize m.
-  instantiate (1 := ltac:(clear dependent m)).
-  lazymatch goal with |- forall (x:?T) (H:?A x), ?B x => change (@Lift1Prop.impl1 T A B) end.
-  cancel. reflexivity.
-  rewrite <-H2 in H3. clear dependent m. rename m0 into m. rename H3 into H0.
-
-  eexists.
-  subst l; eexists.
-  eexists.
-  eexists.
-  eexists.
-  eexists.
-  eexists.
-  eexists.
-
-  change (BinIntDef.Z.to_nat 1) with 1%nat.
-  unfold Semantics.store.
-  rewrite split_combine.
-  unshelve erewrite (get_sep a_addr a); shelve_unifiable. reflexivity.
-  revert H0. generalize m.
-  instantiate (1 := ltac:(clear dependent m)).
-  lazymatch goal with |- forall (x:?T) (H:?A x), ?B x => change (@Lift1Prop.impl1 T A B) end.
-  cancel. reflexivity.
-  intros.
-  unshelve (let pf := open_constr:(put_sep a_addr a b _ m _) in pose proof pf); shelve_unifiable.
-  revert H0.
-  generalize m.
-  instantiate (1 := ltac:(clear dependent m)).
-  lazymatch goal with |- forall (x:?T) (H:?A x), ?B x => change (@Lift1Prop.impl1 T A B) end.
-  cancel. reflexivity.
-  rewrite <-H1 in H2. clear dependent m. rename m0 into m. rename H2 into H0.
-
-  eexists.
-  eexists.
-  eexists.
-  eexists.
-  eexists.
-  eexists.
-  assumption.
-  eexists.
+  intros. rename H0 into Hm.
+  repeat t.
 Qed.
   
